---
title: SICP: Exercise 1.13
---

Prove that =Fib(n)= is the closest integer to

\begin{equation}
\phi^n/{\sqrt 5}
\end{equation}

where
\begin{equation}
\phi = \frac{1 + \sqrt 5}{2}
\end{equation}

Hint: Let

\begin{equation}
\psi = \frac{1 - \sqrt 5}{2}
\end{equation}

Use induction and the definition of the Fibonacci numbers to prove that
\begin{equation}
Fib(n) = \frac{\phi^n - \psi^n}{\sqrt 5}
\end{equation}

* Solution

Let's start by using induction to prove the proposed equation for =Fib(n)=.

Proof by induction requires to steps:
1. The base case. We need to prove =Fib(0)= holds.
2. The inductive case. With the premis that =Fib(n)= holds, we need to prove that =Fib(n+1)= holds.

This is the solution for 1.

\begin{equation}
Fib(0) = \frac{\phi^0 - \psi^0}{\sqrt 5}
\end{equation}
\begin{equation}
0 = \frac{\phi^0 - \psi^0}{\sqrt 5}
\end{equation}
\begin{equation}
0 = \frac{1 - 1}{\sqrt 5}
\end{equation}
\begin{equation}
0 = \frac{0}{\sqrt 5}
\end{equation}
\begin{equation}
0 = 0
\end{equation}

That is, we just proved it holds for the base case. Next comes the solution for 2.

\begin{equation}
Fib(n+1) = Fib(n-1) + Fib(n)
\end{equation}

We don't know what =Fib(n+1)= looks like, but we know what =Fib(n)= does so we are going to rephrase that equation as

\begin{equation}
Fib(n) = Fib(n+1) - Fib(n-1)
\end{equation}

And then do some algebra

\begin{equation}
\frac{\phi^n - \psi^n}{\sqrt 5} = \frac{\phi^{n+1} - \psi^{n+1}}{\sqrt 5} - (\frac{\phi^{n-1} - \psi^{n-1}}{\sqrt 5})
\end{equation}

\begin{equation}
\frac{\phi^n - \psi^n}{\sqrt 5} = \frac{\phi^{n+1} - \psi^{n+1} -\phi^{n-1} + \psi^{n-1}}{\sqrt 5}
\end{equation}

Multiplying all the equation by √5 and reducing we obtain

\begin{equation}
\phi^n - \psi^n = \phi^n (\phi - \frac{1}{\phi}) - \psi^n (\psi - \frac{1}{\psi})
\end{equation}

In order to prove the equation above, it's enough to prove that

\begin{equation}
\phi - \frac{1}{\phi} = 1
\end{equation}

or

\begin{equation}
\phi^2 - 1 = \phi
\end{equation}

and that

\begin{equation}
\psi - \frac{1}{\psi} = 1
\end{equation}

or

\begin{equation}
\psi^2 - 1 = \psi
\end{equation}

First the ϕ case

\begin{equation}
\frac{1 + \sqrt 5}{2} - \frac{1}{\frac{1 + \sqrt 5}{2}} = 1
\end{equation}

\begin{equation}
\frac{1 + \sqrt 5}{2} - \frac{2}{1 + \sqrt 5} = 1
\end{equation}

\begin{equation}
\frac{(1 + \sqrt 5)^2 - 4}{2 + 2\sqrt 5} = 1
\end{equation}

\begin{equation}
\frac{1 + 2\sqrt 5 + 5 - 4}{2 + 2\sqrt 5} = 1
\end{equation}

\begin{equation}
\frac{2 + 2\sqrt 5}{2 + 2\sqrt 5} = 1
\end{equation}

\begin{equation}
1 = 1
\end{equation}

Now the ᴪ case

\begin{equation}
\frac{1 - \sqrt 5}{2} - \frac{1}{\frac{1 - \sqrt 5}{2}} = 1
\end{equation}

\begin{equation}
\frac{(1 - \sqrt 5)^2 - 4}{2 - 2\sqrt 5} = 1
\end{equation}

\begin{equation}
\frac{1 - 2\sqrt 5 + 5 - 4}{2 - 2\sqrt 5} = 1
\end{equation}

\begin{equation}
\frac{2 - 2\sqrt 5}{2 - 2\sqrt 5} = 1
\end{equation}

\begin{equation}
1 = 1
\end{equation}

And with that we have proven that effectively

\begin{equation}
Fib(n) = \frac{\phi^n - \psi^n}{\sqrt 5}
\end{equation}

Now, returning to the first question that asked to prove that =Fib(n)= is the closest integer to

\begin{equation}
\phi^n/{\sqrt 5}
\end{equation}

We have to prove that

\begin{equation}
\lvert Fib(n) - \frac{\phi^n}{\sqrt 5} \rvert < \frac{1}{2}
\end{equation}

that is, =ϕ^n/√5= is, at most, a half away of =Fib(n)=, and since =Fib(n+1)= is an integer greater thatn =Fib(n)=, then that proof has to be enough.

But we've proven that =Fib(n)= is =(ϕ^n-ψ^n)/√5=

\begin{equation}
\lvert \frac{\phi^n - \psi^n}{\sqrt 5} - \frac{\phi^n}{\sqrt 5} \rvert < \frac{1}{2}
\end{equation}

\begin{equation}
\lvert \frac{- \psi^n}{\sqrt 5} \rvert < \frac{1}{2}
\end{equation}

Now, let's use induction again to prove it.

Here's the base case

\begin{equation}
\lvert \frac{- \psi^0}{\sqrt 5} \rvert < \frac{1}{2}
\end{equation}

\begin{equation}
\lvert \frac{- 1}{\sqrt 5} \rvert < \frac{1}{2}
\end{equation}

\begin{equation}
\frac{1}{\sqrt 5} < \frac{1}{2}
\end{equation}

\begin{equation}
2 < \sqrt 5
\end{equation}

which is true.

And here's the inductive case

\begin{equation}
\lvert \frac{- \psi^{n+1}}{\sqrt 5} \rvert < \frac{1}{2}
\end{equation}

\begin{equation}
\lvert \frac{- \psi^n}{\sqrt 5} \psi \rvert < \frac{1}{2}
\end{equation}

Now, we know

\begin{equation}
\lvert \frac{- \psi^n}{\sqrt 5} \rvert < \frac{1}{2}
\end{equation}

but let's suppose that

\begin{equation}
\lvert \frac{- \psi^n}{\sqrt 5} \rvert = \frac{1}{2}
\end{equation}

if that's the case we'll get

\begin{equation}
\lvert -\frac{1}{2} \frac{1 - \sqrt 5}{2} \rvert < \frac{1}{2}
\end{equation}

\begin{equation}
\lvert \frac{\sqrt 5 - 1}{4} \rvert < \frac{1}{2}
\end{equation}

\begin{equation}
\lvert \sqrt 5 - 1 \rvert < 2
\end{equation}

which is true, then, it has to be also true in the same case that

\begin{equation}
\lvert \frac{- \psi^n}{\sqrt 5} \rvert < \frac{1}{2}
\end{equation}

since that number being less than a half is going to cause the when multiplied by ψ the result is going to be also less than a half.

Hence, we've proved that

\begin{equation}
\lvert \frac{- \psi^n}{\sqrt 5} \rvert < \frac{1}{2}
\end{equation}

and by that, that =Fib(n)= has to be the closest integer to =ϕ^n/√5=.
